GVN3.v
@@ -1,0 +1,343 @@
+Require Import Bool.
+Require Import Sorting.Permutation.
+Require Import Omega.
+Require Import sflib.
+Require Import Lia.
+
+Require Import Common.
+Require Import Value.
+Require Import Lang.
+Require Import Memory.
+Require Import State.
+Require Import LoadStore.
+Require Import SmallStep.
+Require Import Refinement.
+Require Import SmallStepRefinement.
+Require Import Reordering.
+Require Import GVN1.
+
+Module Ir.
+
+Module GVN3.
+
+
+(* 3nd condition of replacing p with q:
+   If p and q are both computed by the gep inbounds with same
+   base pointer, it is valid to replace p with q. *)
+Definition eqprop_valid3 (m:Ir.Memory.t) (p q:Ir.val) :=
+  exists p0 idx1 idx2 ty1 ty2,
+    p = Ir.SmallStep.gep p0 idx1 ty1 m true /\
+    q = Ir.SmallStep.gep p0 idx2 ty2 m true.
+
+
+
+(*********************************************************
+ Important property of eqprop_valid3:
+  If eqprop_valid3 p q holds, and `icmp eq p, q` evaluates
+    to true, then p and q are exactly the same pointer.
+ *********************************************************)
+
+Lemma twos_compl_twos_compl_add_OPAQUED_PTRSZ:
+  forall n x,
+    Ir.SmallStep.twos_compl (Ir.SmallStep.twos_compl_add n x Ir.SmallStep.OPAQUED_PTRSZ) Ir.PTRSZ =
+    Ir.SmallStep.twos_compl_add n x Ir.SmallStep.OPAQUED_PTRSZ.
+Proof.
+  intros.
+  rewrite Ir.GVN1.OPAQUED_PTRSZ_PTRSZ.
+  unfold Ir.SmallStep.twos_compl_add.
+  unfold Ir.SmallStep.twos_compl.
+  rewrite Nat.mod_mod. reflexivity.
+  apply shiftl_2_nonzero.
+Qed.
+
+Theorem gep_never_returns_num:
+  forall v p idx ty m inb
+    (HGEP1:Ir.SmallStep.gep p idx ty m inb = v),
+    ~exists n, v = Ir.num n.
+Proof.
+  intros.
+  unfold Ir.SmallStep.gep in HGEP1.
+  intros HH.
+  inv HH.
+  des_ifs.
+Qed.
+
+(* I had to split the big theorem into lemmas due to
+   Coq bug - Coq does not terminate processing of 'Qed.', due to unknown reason :( *)
+Lemma eqprop_valid3_after_icmpeq_true_log:
+  forall md st st' r ptrty op1 op2 p1 p2 e l0 o0 idx1 ty1 idx2 ty2
+    (HWF:Ir.Config.wf md st)
+    (HINST:Some (Ir.Inst.iicmp_eq r ptrty op1 op2) = Ir.Config.cur_inst md st)
+    (HOP1:Some (Ir.ptr p1) = Ir.Config.get_val st op1)
+    (HOP2:Some (Ir.ptr p2) = Ir.Config.get_val st op2)
+    (* geps *)
+    (HGEP1:(Ir.ptr p1) = Ir.SmallStep.gep (Ir.plog l0 o0) idx1 ty1 (Ir.Config.m st) true)
+    (HGEP2:(Ir.ptr p2) = Ir.SmallStep.gep (Ir.plog l0 o0) idx2 ty2 (Ir.Config.m st) true)
+    (* have a small step *)
+    (HSTEP:Ir.SmallStep.sstep md st (Ir.SmallStep.sr_success e st'))
+    (* p1 == p2 is true *)
+    (HTRUE:Some (Ir.num 1) = Ir.Config.get_val st' (Ir.opreg r)),
+
+    p1 = p2.
+Proof.
+  intros.
+
+  assert (HS:Ir.Config.s st <> []).
+  {
+    unfold Ir.Config.cur_inst in HINST.
+    unfold Ir.Config.cur_fdef_pc in HINST.
+    des_ifs.
+  }
+
+  inv HSTEP.
+  { inv HISTEP; try congruence.
+    { unfold Ir.SmallStep.inst_det_step in HNEXT.
+      rewrite <- HINST in HNEXT.
+      rewrite <- HOP1, <- HOP2 in HNEXT.
+      unfold Ir.SmallStep.icmp_eq_ptr in HNEXT.
+      unfold Ir.SmallStep.gep in *.
+      des_ifs.
+      {
+        rewrite Ir.Reordering.get_val_update_reg_and_incrpc in HTRUE.
+        unfold Ir.Config.get_val in HTRUE.
+        rewrite Ir.Config.get_rval_update_rval_id in HTRUE.
+        inv HTRUE.
+        des_ifs.
+        rewrite Nat.eqb_eq in Heq3. congruence. assumption.
+      }
+      {
+        rewrite Ir.Reordering.get_val_update_reg_and_incrpc in HTRUE.
+        unfold Ir.Config.get_val in HTRUE.
+        rewrite Ir.Config.get_rval_update_rval_id in HTRUE.
+        inv HTRUE.
+        des_ifs.
+      }
+    }
+    { rewrite <- HINST in HCUR.
+      inv HCUR.
+      rewrite <- HOP1 in HOP0. inv HOP0.
+      rewrite <- HOP2 in HOP3. inv HOP3.
+      unfold Ir.SmallStep.gep in *.
+      unfold Ir.SmallStep.icmp_eq_ptr_nondet_cond in *.
+      des_ifs; rewrite Nat.eqb_refl in HNONDET; inv HNONDET.
+    }
+  }
+  { apply Ir.Config.cur_inst_not_cur_terminator in HINST.
+    unfold Ir.SmallStep.t_step in HTSTEP. rewrite <- HINST in HTSTEP.
+    congruence.
+  }
+Qed.
+
+Definition OPAQUED_MEMSZ := Ir.SmallStep.locked nat Ir.MEMSZ.
+Lemma OPAQUED_MEMSZ_MEMSZ:
+  OPAQUED_MEMSZ = Ir.MEMSZ.
+Proof.
+  intros. unfold OPAQUED_MEMSZ. unfold Ir.SmallStep.locked.
+  des_ifs.
+Qed.
+
+(* due to Coq bug, I made a separated lemmax *)
+Lemma gep_helper_small:
+  forall n l o x1 x3 st p0 n'1
+(HVAL2 : Ir.SmallStep.gep (Ir.pphy n l o) x1 x3 (Ir.Config.m st) true =
+          Ir.ptr p0)
+(Heqn'1: n'1 =
+           Ir.SmallStep.twos_compl_add n (x1 * Ir.ty_bytesz x3)
+             Ir.SmallStep.OPAQUED_PTRSZ),
+  p0 = Ir.pphy n'1 (n::n'1::l) o.
+Proof.
+  intros. unfold Ir.SmallStep.gep in HVAL2. des_ifs.
+Qed.
+
+Lemma gep_helper:
+  forall n l o x1 x3 x0 x2 st p0 p st' r e md
+(HVAL2 : Ir.SmallStep.gep (Ir.pphy n l o) x1 x3 (Ir.Config.m st) true =
+          Ir.ptr p0)
+(HVAL1 : Ir.SmallStep.gep (Ir.pphy n l o) x0 x2 (Ir.Config.m st) true =
+          Ir.ptr p)
+(HTRUE : Some (Ir.num 1) = Ir.Config.get_val st' (Ir.opreg r))
+(HNEXT : Some (Ir.SmallStep.sr_success e st') =
+          match Ir.SmallStep.icmp_eq_ptr p p0 (Ir.Config.m st) with
+          | Some b =>
+              Some
+                (Ir.SmallStep.sr_success Behaviors.Ir.e_none
+                   (Ir.SmallStep.update_reg_and_incrpc md st r
+                      (Ir.SmallStep.to_num b)))
+          | None => None
+          end)
+(HS : Ir.Config.s st <> []),
+    Ir.ptr p = Ir.ptr p0.
+Proof.
+  intros.
+  eapply gep_helper_small in HVAL2; try reflexivity.
+  eapply gep_helper_small in HVAL1; try reflexivity.
+  rewrite HVAL1, HVAL2 in HNEXT.
+  unfold Ir.SmallStep.icmp_eq_ptr in HNEXT.
+  unfold Ir.SmallStep.p2N in HNEXT.
+  rewrite twos_compl_twos_compl_add_OPAQUED_PTRSZ in HNEXT.
+  inversion HNEXT.
+  rewrite H1 in HTRUE.
+  rewrite Ir.Reordering.get_val_update_reg_and_incrpc in HTRUE.
+  unfold Ir.Config.get_val in HTRUE.
+  rewrite Ir.Config.get_rval_update_rval_id in HTRUE.
+  inversion HTRUE.
+  destruct (Ir.SmallStep.twos_compl_add n (x0 * Ir.ty_bytesz x2) Ir.SmallStep.OPAQUED_PTRSZ =?
+         Ir.SmallStep.twos_compl_add n (x1 * Ir.ty_bytesz x3) Ir.SmallStep.OPAQUED_PTRSZ)
+           eqn:Heq; try congruence.
+  rewrite Nat.eqb_eq in Heq. rewrite HVAL1, HVAL2, Heq.
+  reflexivity.
+  assumption.
+Admitted. (* This is really strange.. Why Qed never ends? *)
+
+
+Theorem eqprop_valid3_after_icmpeq_true:
+  forall md st st' r ptrty op1 op2 v1 v2 e
+    (HWF:Ir.Config.wf md st)
+    (HINST:Some (Ir.Inst.iicmp_eq r ptrty op1 op2) = Ir.Config.cur_inst md st)
+    (HOP1:Some v1 = Ir.Config.get_val st op1)
+    (HOP2:Some v2 = Ir.Config.get_val st op2)
+    (* eqprop_valid3 holds *)
+    (HEQPROP:eqprop_valid3 (Ir.Config.m st) v1 v2)
+    (* have a small step *)
+    (HSTEP:Ir.SmallStep.sstep md st (Ir.SmallStep.sr_success e st'))
+    (* p1 == p2 is true *)
+    (HTRUE:Some (Ir.num 1) = Ir.Config.get_val st' (Ir.opreg r)),
+
+    v1 = v2.
+Proof.
+  intros.
+  assert (HS:Ir.Config.s st <> []).
+  {
+    unfold Ir.Config.cur_inst in HINST.
+    unfold Ir.Config.cur_fdef_pc in HINST.
+    des_ifs.
+  }
+
+  inv HSTEP.
+  { inv HISTEP; try congruence.
+    { inv HEQPROP.
+      inv H. inv H0. inv H. inv H0. inv H.
+      destruct x.
+      { destruct (Ir.SmallStep.gep (Ir.plog b n) x0 x2 (Ir.Config.m st) true) eqn:HVAL1;
+          destruct (Ir.SmallStep.gep (Ir.plog b n) x1 x3 (Ir.Config.m st) true) eqn:HVAL2;
+        try (apply gep_never_returns_num in HVAL1;
+             exfalso; apply HVAL1; eexists; reflexivity);
+        try (apply gep_never_returns_num in HVAL2;
+             exfalso; apply HVAL2; eexists; reflexivity).
+        { exploit eqprop_valid3_after_icmpeq_true_log.
+          { eassumption. }
+          { eassumption. }
+          { eassumption. }
+          { eassumption. }
+          { rewrite HVAL1. reflexivity. }
+          { rewrite HVAL2. reflexivity. }
+          { eapply Ir.SmallStep.ss_inst.
+            eapply Ir.SmallStep.s_det.
+            eassumption. }
+          { eassumption. }
+          intros HH. congruence.
+        }
+        { unfold Ir.SmallStep.inst_det_step in HNEXT.
+          rewrite <- HINST in HNEXT.
+          rewrite <- HOP2 in HNEXT. des_ifs.
+          rewrite Ir.Reordering.get_val_update_reg_and_incrpc in HTRUE.
+          unfold Ir.Config.get_val in HTRUE.
+          rewrite Ir.Config.get_rval_update_rval_id in HTRUE.
+          inv HTRUE. assumption.
+        }
+        { unfold Ir.SmallStep.inst_det_step in HNEXT.
+          rewrite <- HINST in HNEXT.
+          rewrite <- HOP1 in HNEXT. des_ifs.
+          rewrite Ir.Reordering.get_val_update_reg_and_incrpc in HTRUE.
+          unfold Ir.Config.get_val in HTRUE.
+          rewrite Ir.Config.get_rval_update_rval_id in HTRUE.
+          inv HTRUE. assumption.
+        }
+        { unfold Ir.SmallStep.inst_det_step in HNEXT.
+          rewrite <- HINST in HNEXT.
+          rewrite <- HOP2 in HNEXT. des_ifs.
+        }
+      }
+      { (* phy. *)
+        unfold Ir.SmallStep.inst_det_step in HNEXT.
+        rewrite <- HINST in HNEXT.
+        rewrite <- HOP1, <- HOP2 in HNEXT.
+
+        destruct (Ir.SmallStep.gep (Ir.pphy n l o) x0 x2 (Ir.Config.m st) true) eqn:HVAL1;
+          destruct (Ir.SmallStep.gep (Ir.pphy n l o) x1 x3 (Ir.Config.m st) true) eqn:HVAL2;
+        try (apply gep_never_returns_num in HVAL1;
+             exfalso; apply HVAL1; eexists; reflexivity);
+        try (apply gep_never_returns_num in HVAL2;
+             exfalso; apply HVAL2; eexists; reflexivity).
+        { eapply gep_helper; try eassumption. }
+        { inv HNEXT.
+          rewrite Ir.Reordering.get_val_update_reg_and_incrpc in HTRUE.
+          unfold Ir.Config.get_val in HTRUE.
+          rewrite Ir.Config.get_rval_update_rval_id in HTRUE.
+          inv HTRUE. assumption. }
+        { inv HNEXT.
+          rewrite Ir.Reordering.get_val_update_reg_and_incrpc in HTRUE.
+          unfold Ir.Config.get_val in HTRUE.
+          rewrite Ir.Config.get_rval_update_rval_id in HTRUE.
+          inv HTRUE. assumption. }
+        { reflexivity. }
+      }
+    }
+    { (* well, cannot be nondet... *)
+      rewrite <- HINST in HCUR. inv HCUR.
+      rewrite <- HOP1 in HOP0. inv HOP0.
+      rewrite <- HOP2 in HOP3. inv HOP3.
+      inv HEQPROP.
+      inv H. inv H0. inv H. inv H0. destruct H.
+      destruct x.
+      { assert (HOFS1:exists ofs1, p1 = (Ir.plog b ofs1)).
+        { unfold Ir.SmallStep.gep in H.
+          unfold Ir.SmallStep.gep in H0.
+          unfold Ir.SmallStep.icmp_eq_ptr_nondet_cond in HNONDET.
+          des_ifs; eexists; reflexivity. }
+        assert (HOFS2:exists ofs2, p2 = (Ir.plog b ofs2)).
+        { unfold Ir.SmallStep.gep in H.
+          unfold Ir.SmallStep.gep in H0.
+          unfold Ir.SmallStep.icmp_eq_ptr_nondet_cond in HNONDET.
+          des_ifs; eexists; reflexivity. }
+        inv HOFS1. inv HOFS2.
+        unfold Ir.SmallStep.icmp_eq_ptr_nondet_cond in HNONDET.
+        des_ifs;
+          rewrite Nat.eqb_refl in HNONDET; inv HNONDET.
+      }
+      { assert (HOFS1:exists a1 b1 c1, p1 = (Ir.pphy a1 b1 c1)).
+        { unfold Ir.SmallStep.gep in H.
+          unfold Ir.SmallStep.gep in H0.
+          unfold Ir.SmallStep.icmp_eq_ptr_nondet_cond in HNONDET.
+          des_ifs; eexists; reflexivity. }
+        assert (HOFS2:exists a2 b2 c2, p2 = (Ir.pphy a2 b2 c2)).
+        { unfold Ir.SmallStep.gep in H.
+          unfold Ir.SmallStep.gep in H0.
+          unfold Ir.SmallStep.icmp_eq_ptr_nondet_cond in HNONDET.
+          des_ifs; eexists; reflexivity. }
+        inv HOFS1. inv H1. inv H2.
+        inv HOFS2. inv H1. inv H2.
+        unfold Ir.SmallStep.icmp_eq_ptr_nondet_cond in HNONDET.
+        des_ifs.
+      }
+    }
+  }
+  { (* terminator! *)
+    apply Ir.Config.cur_inst_not_cur_terminator in HINST.
+    unfold Ir.SmallStep.t_step in HTSTEP.
+    rewrite <- HINST in HTSTEP.
+    congruence.
+  }
+Qed.
+
+(*********************************************************
+    Okay, from theorem `eqprop_valid3_after_icmpeq_true`,
+    we can say that two pointers have same value after
+    `p == q` check.
+    It is trivial to have same execution when same value
+    is given, hence not proved.
+ *********************************************************)
+
+End GVN3.
+
+End Ir.
